

Let $n \geq 2$ be an integer, and let a_1, a_2, \dots, a_n be positive real numbers such that $a_1 + a_2 + \dots + a_n = 1$.
Prove that

$$\sum_{k=1}^n \frac{a_k}{1-a_k} (a_1 + a_2 + \dots + a_{k-1})^2 < \frac{1}{3}.$$

$$S_k = a_1 + a_2 + \dots + a_k \quad (S_0 = 0), \quad S_n = 1$$

$$\sum_{k=1}^n \frac{a_k S_{k-1}^2}{1-a_k} < \frac{1}{3}$$

$$\sum_{k=1}^n \frac{a_k S_{k-1}^2}{1-a_k} < \frac{1}{3} \sum_{k=1}^n (S_k^3 - S_{k-1}^3) \quad \text{①} \quad \text{②}$$

$$\sum_{k=1}^n (S_k - S_{k-1}) = 1$$

$$\sum_{k=1}^n (S_k^2 - S_{k-1}^2) = 1$$

$$\sum_{k=1}^n (S_k^3 - S_{k-1}^3) = 1$$

$$\text{let } \alpha = a_k, \quad \beta = S_{k-1}$$

$$\alpha + \beta = S_k \leq 1 \quad \therefore \alpha + \beta \leq 1 \quad \text{③}$$

$$\text{If } \frac{\alpha S_{k-1}^2}{1-a_k} < \frac{S_k^3 - S_{k-1}^3}{3}, \quad \text{then } \sum_{k=1}^n \frac{a_k S_{k-1}^2}{1-a_k} < \frac{1}{3} \sum_{k=1}^n (S_k^3 - S_{k-1}^3).$$

$$\frac{\alpha \beta^2}{1-\alpha} < \frac{(\alpha+\beta)^3 - \beta^3}{3} = \frac{\alpha^3 + 3\alpha^2\beta + 3\alpha\beta^2}{3}$$

$$\frac{\alpha \beta^2}{1-\alpha} - \alpha \beta^2 < \frac{\alpha^3 + 3\alpha^2\beta}{3}$$

$$\frac{\alpha^2 \beta^2}{1-\alpha} < \frac{\alpha^3 + 3\alpha^2\beta}{3}$$

$$\frac{\beta^2}{1-\alpha} < \frac{\alpha + 3\beta}{3}$$

$$\beta \leq 1-\alpha$$

$$\frac{\beta^2}{1-\alpha} \leq \beta$$

$$\frac{\beta^2}{1-\alpha} \leq \beta < \frac{\alpha}{3} + \beta$$

□

Let $n \geq 2$ be an integer, and let a_1, a_2, \dots, a_n be positive real numbers such that $a_1 + a_2 + \dots + a_n = 1$.
Prove that

$$\sum_{k=1}^n \frac{a_k}{1-a_k} (a_1 + a_2 + \dots + a_{k-1})^2 < \frac{1}{3}.$$

$$\text{let } S_k = a_1 + a_2 + \dots + a_k$$

$$\sum_{k=1}^n \frac{a_k S_{k-1}^2}{1-a_k} < \frac{1}{3}$$

$$k \geq 1 \quad 1 - a_k > 0$$

$$\sum_{k=1}^n \frac{a_k s_{k-1}^2}{1-a_k} < \frac{1}{3} \sum_{k=1}^n (s_k^2 - s_{k-1}^2)$$

If $\frac{a_k s_{k-1}^2}{1-a_k} < \frac{s_k^2 - s_{k-1}^2}{3}$, then we use our inequality.

$$\text{let } \alpha \geq a_k, \quad \beta \geq s_{k-1}$$

$$\frac{\boxed{\alpha \beta^2}}{1-\alpha} < \frac{(\alpha+\beta)^2 - \beta^2}{3} = \frac{\alpha^2 + 2\alpha\beta}{3}$$